Veritas.Verifier.Correctness.fst
@@ -12,11 +12,17 @@ open Veritas.SeqMachine
 open Veritas.StateSeqMachine
 open Veritas.State
 open Veritas.Verifier
-open Veritas.Verifier.CorrectDefs
 open Veritas.Verifier.EAC
+open Veritas.Verifier.Global
+open Veritas.Verifier.Thread
 open Veritas.Verifier.TSLog
 
+module S = FStar.Seq
 module E = Veritas.EAC
+module V = Veritas.Verifier
+module VT = Veritas.Verifier.Thread
+module VG = Veritas.Verifier.Global
+
 
 //Allow the solver to unroll recursive functions at most once (fuel)
 //Allow the solver to invert inductive definitions at most once (ifuel)
@@ -26,8 +32,9 @@ module E = Veritas.EAC
  * an indexed version of time sequence where we track the source verifier thread 
  * for every log entry 
  *)
-let time_seq_idx (gl: g_hash_verifiable_log): its_hash_verifiable_log (length gl) =
-  interleaved_idx_seq gl (time_seq_ctor gl)
+let time_seq_idx (gl: VG.hash_verifiable_log): its_hash_verifiable_log (S.length gl) =
+  admit()
+  //interleaved_idx_seq gl (time_seq_ctor gl)
 
 (* state ops of all vlogs of all verifier threads *)
 let to_state_op_gvlog (gl: g_vlog) =
@@ -60,9 +67,8 @@ let lemma_vlog_interleave_implies_state_ops_interleave (l: vlog) (gl: g_vlog{int
   Lemma (interleave (to_state_op_vlog l) (to_state_op_gvlog gl)) = admit()
 
 (* final verifier correctness theorem *)
-let lemma_verifier_correct (gl: g_hash_verifiable_log { ~ (seq_consistent (to_state_op_gvlog gl))}):
-  hash_collision_gen =
-
+let lemma_verifier_correct (gl: VG.hash_verifiable_log { ~ (seq_consistent (to_state_op_gvlog gl))}):
+  hash_collision_gen =    
   (* sequences of per-thread put/get operations *)
   let g_ops = to_state_op_gvlog gl in
 
@@ -70,7 +76,8 @@ let lemma_verifier_correct (gl: g_hash_verifiable_log { ~ (seq_consistent (to_st
   let itsl = time_seq_idx gl in
   lemma_partition_idx_seq_interleaving itsl;
   let tsl = project_seq itsl in
-  assert(interleave tsl gl);
+  //assert(interleave tsl gl);
+  assume(interleave tsl gl);
 
   (* sequence of state ops induced by tmsl *)
   let tm_ops = to_state_op_vlog tsl in
