Veritas.Verifier.Global.fst
@@ -1,0 +1,17 @@
+module Veritas.Verifier.Global
+
+(* aggregate hadd over all verifier threads *)
+let hadd (gl: verifiable_log): ms_hash_value =
+  let th = fun (tl:VT.verifiable_log) -> (thread_hadd (t_verify (fst tl) (snd tl))) in
+  let f = fun (tl:VT.verifiable_log) (h:ms_hash_value) -> (ms_hashfn_agg (th tl) h) in
+  reduce empty_hash_value f (verifiable_threads gl)
+
+(* aggregate hadd over all verifier threads *)
+let hevict (gl: verifiable_log): ms_hash_value =
+  let th = fun (tl:VT.verifiable_log) -> (thread_hevict (t_verify (fst tl) (snd tl))) in
+  let f = fun (tl:VT.verifiable_log) (h:ms_hash_value) -> (ms_hashfn_agg (th tl) h) in
+  reduce empty_hash_value f (verifiable_threads gl)
+
+let clock (gl: verifiable_log) (i: sseq_index gl): timestamp = admit()
+
+let time_seq_ctor (gl: verifiable_log): (interleave_ctor gl) = admit()
