Veritas.Verifier.Global.fsti
@@ -1,0 +1,57 @@
+module Veritas.Verifier.Global
+
+open Veritas.Interleave
+open Veritas.MultiSetHash
+open Veritas.Verifier
+open Veritas.Verifier.Thread
+
+open FStar.Seq
+open Veritas.SeqAux
+
+module MH = Veritas.MultiSetHash
+module V = Veritas.Verifier
+module VT = Veritas.Verifier.Thread
+
+(* Full collection of verifier logs one per thread *)
+let g_vlog = (gl:seq vlog{length gl > 0})
+
+(* a slightly different view of verifier log obtained by
+ * attaching a tid (index) to each thread verifier log *)
+let g_tid_vlog (gl: g_vlog): seq thread_id_vlog = 
+  attach_index gl
+
+(* globally verifiable logs: every thread-level log is verifiable *)
+let verifiable (gl: g_vlog) = 
+  all VT.verifiable (g_tid_vlog gl)
+
+(* Refinement type of logs that are verifiable *)
+let verifiable_log = gl:g_vlog{verifiable gl}
+
+(* verifiable thread-level logs *)
+let verifiable_threads (gl: verifiable_log): seq VT.verifiable_log
+  = seq_refine VT.verifiable (g_tid_vlog gl)
+
+(* add-set hash over all verifier threads *)
+val hadd (gl: verifiable_log): ms_hash_value
+
+(* hash of evict set over all verifier threads *)
+val hevict (gl: verifiable_log): ms_hash_value
+
+(* a verifiable log is hash verifiable if add and evict set hashes are equal *)
+let hash_verifiable (gl: verifiable_log): bool = 
+  hadd gl = hevict gl
+
+let hash_verifiable_log = gl:verifiable_log{hash_verifiable gl}
+
+(* 
+ * return the clock of a particular log entry. the index i here 
+ * is a pair that identifies the verifier thread and an entry
+ * in the thread log
+ *)
+val clock (gl: verifiable_log) (i: sseq_index gl): timestamp
+
+(* time ordered interleaving of a verifier logs. the "constructor" of the 
+ * interleaving contains both the sequence and the proof of the interleaving
+ * which helps track the lineage of each entry in the interleaved sequence *)
+val time_seq_ctor (gl: verifiable_log): (interleave_ctor gl)
+
