Veritas.Verifier.Thread.fst
@@ -1,0 +1,47 @@
+module Veritas.Verifier.Thread
+
+let rec lemma_verifiable_implies_prefix_verifiable_aux
+  (tl:verifiable_log) (i:nat{i <= length tl}):
+  Lemma (requires (True))
+        (ensures (verifiable (prefix tl i)))
+        (decreases (length tl)) = 
+  let n = length tl in
+  if i = n then ()
+  else lemma_verifiable_implies_prefix_verifiable_aux (prefix tl (n - 1)) i
+
+let lemma_verifiable_implies_prefix_verifiable = lemma_verifiable_implies_prefix_verifiable_aux
+
+(* the clock of a verifier is monotonic *)
+let rec lemma_clock_monotonic_aux (tl:verifiable_log) (i:idx tl):
+  Lemma (requires(True))
+        (ensures (clock tl i `ts_leq` clock tl (length tl - 1)))
+  (decreases (length tl))
+        =
+  let n = length tl in
+  if n = 0 then ()
+  else if i = n - 1 then ()
+  else
+    let tl' = prefix tl (n - 1) in
+    lemma_clock_monotonic_aux tl' i
+
+let lemma_clock_monotonic (tl: verifiable_log) (i:idx tl) (j:idx tl{j >= i}): 
+  Lemma (clock tl i `ts_leq` clock tl j) = 
+  let tlj = prefix tl (j + 1) in
+  lemma_clock_monotonic_aux tlj i
+
+let rec lemma_thread_id_state_aux (tl: verifiable_log):
+  Lemma (requires True)
+        (ensures (V.thread_id_of (verify tl) = thread_id_of tl)) 
+        (decreases (length tl)) = 
+  let n = length tl in
+  if n = 0 then ()
+  else
+    lemma_thread_id_state_aux (prefix tl (n - 1))
+
+let lemma_thread_id_state = lemma_thread_id_state_aux
+
+let lemma_requires_key_in_store 
+  (tl: verifiable_log) 
+  (i:idx tl{requires_key_in_store (index tl i)}):
+  Lemma (store_contains (store_idx tl i) (V.key_of (index tl i))) =
+  admit()
