Veritas.Verifier.Thread.fsti
@@ -1,0 +1,91 @@
+module Veritas.Verifier.Thread
+
+open Veritas.MultiSetHash
+open Veritas.SeqAux
+open Veritas.Verifier
+
+module S = FStar.Seq
+module SA = Veritas.SeqAux
+module V = Veritas.Verifier
+
+(*
+ * an indexed vlog attaches an nat index to a vlog
+ * indicating the id of the verifier thread processing
+ * the log
+ *)
+let thread_id_vlog = thread_id & vlog
+
+(* thread id of the indexed vlog *)
+let thread_id_of (tl: thread_id_vlog): nat = fst tl
+
+(* vlog of an indexed vlog *)
+let vlog_of (tl: thread_id_vlog): vlog = snd tl
+
+let length (tl: thread_id_vlog): nat =
+  S.length (vlog_of tl)
+
+let idx (tl: thread_id_vlog) = i:nat{i < length tl}
+
+let index (tl: thread_id_vlog) (i:idx tl): vlog_entry =
+  S.index (vlog_of tl) i
+
+let append1 (tl: thread_id_vlog) (e: vlog_entry): thread_id_vlog =
+  (thread_id_of tl), (SA.append1 (vlog_of tl) e)
+
+let prefix (tl: thread_id_vlog) (i:nat{i <= length tl}): thread_id_vlog =
+  (thread_id_of tl), (SA.prefix (vlog_of tl) i)
+
+let verify (tl:thread_id_vlog): V.vtls =
+  t_verify (thread_id_of tl) (vlog_of tl)
+
+let verifiable (tl: thread_id_vlog): bool =
+  Valid? (verify tl)
+
+let verifiable_log = tl: thread_id_vlog {verifiable tl}
+
+(* if a thread log is verifiable, its prefix is verifiable *)
+val lemma_verifiable_implies_prefix_verifiable
+  (tl:verifiable_log) (i:nat{i <= length tl}):
+  Lemma (requires (True))
+        (ensures (verifiable (prefix tl i)))
+        [SMTPat (prefix tl i)]
+
+(* clock after processing the i'th entry *)
+let clock (tl:verifiable_log) (i:idx tl): timestamp =
+  Valid?.clk (verify (prefix tl (i + 1)))
+
+(* clock is monotonic *)
+val lemma_clock_monotonic (tl: verifiable_log) (i:idx tl) (j:idx tl{j >= i}): 
+  Lemma (clock tl i `ts_leq` clock tl j)
+
+(* the thread id in the state is always the one specified in the parameter *)
+val lemma_thread_id_state (tl: verifiable_log):
+  Lemma (V.thread_id_of (verify tl) = thread_id_of tl)
+
+(* these log entries require the store contain the key_of e, otherwise result in a failure *)
+let requires_key_in_store (e:vlog_entry): bool = 
+  match e with
+  | Get _ _ -> true
+  | Put _ _ -> true
+  | EvictM _ _ -> true
+  | EvictB _ _ -> true
+  | EvictBM _ _ _ -> true
+  | _ -> false
+
+(* the store after processing a log *)
+let store (tl:verifiable_log): vstore = 
+  Valid?.st (verify tl)
+
+(* the store after processing i entries *)
+let store_idx (tl: verifiable_log) (i: idx tl): vstore = 
+  store (prefix tl i)
+
+(* 
+ * if the (i+1)'th entry requires the key to be in the store, then the verifier store 
+ * contains the key after processing i entries 
+ *)
+val lemma_requires_key_in_store 
+  (tl: verifiable_log) 
+  (i:idx tl{requires_key_in_store (index tl i)}):
+  Lemma (store_contains (store_idx tl i) (V.key_of (index tl i)))
+
